<?xml version='1.0'?>
<!--

 Licensed to the Apache Software Foundation (ASF) under one
 or more contributor license agreements.  See the NOTICE file
 distributed with this work for additional information
 regarding copyright ownership.  The ASF licenses this file
 to you under the Apache License, Version 2.0 (the
 "License"); you may not use this file except in compliance
 with the License.  You may obtain a copy of the License at

   http://www.apache.org/licenses/LICENSE-2.0

 Unless required by applicable law or agreed to in writing,
 software distributed under the License is distributed on an
 "AS IS" BASIS, WITHOUT WARRANTIES OR CONDITIONS OF ANY
 KIND, either express or implied.  See the License for the
 specific language governing permissions and limitations
 under the License.

-->

<rdf:RDF xmlns="http://clerezza.org/2009/09/hierarchy#"
	xml:base="http://clerezza.org/2009/09/hierarchy"
	xmlns:hierarchy="http://clerezza.org/2009/09/hierarchy#"
	xmlns:xsd="http://www.w3.org/2001/XMLSchema#"
	xmlns:rdfs="http://www.w3.org/2000/01/rdf-schema#"
	xmlns:rdf="http://www.w3.org/1999/02/22-rdf-syntax-ns#"
	xmlns:owl="http://www.w3.org/2002/07/owl#"
	xmlns:dc="http://purl.org/dc/elements/1.1/"
	xmlns:dbt="http://discobits.org/ontology#">

	<owl:Ontology rdf:about="http://clerezza.org/2009/09/hierarchy#">
		<dc:title>Clerezza Ontology for Hierarchical Structure</dc:title>
	</owl:Ontology>

    <!-- Classes -->

	<owl:Class rdf:about="#Collection">
		<rdfs:comment>An ordered  collection of members. The URI of a Collection
			must end with a slash ('/').</rdfs:comment>
	</owl:Class>

	<owl:Class rdf:about="#Page">
		<rdfs:comment>A titled content that is typically displayed in a web browser
			without being a part of a containing entity.</rdfs:comment>
		<rdfs:subClassOf rdf:resource="dbt:TitledContent" />
	</owl:Class>

	<owl:ObjectProperty rdf:about="#members">
        <rdfs:comment>Points to a list of Resources.</rdfs:comment>
        <rdfs:domain rdf:resource="#Collection"/>
        <rdfs:range rdf:resource="rdf:List"/>
    </owl:ObjectProperty>

	<owl:ObjectProperty rdf:about="#membersNumber">
        <rdfs:comment>Points from a collection to an integer that states the
			number of members in the collection.</rdfs:comment>
        <rdfs:domain rdf:resource="#Collection"/>
        <rdfs:range rdf:resource="xsd:int"/>
    </owl:ObjectProperty>

	<owl:ObjectProperty rdf:about="#parent">
        <rdfs:comment>Points from a resource to its parent collection.</rdfs:comment>
        <rdfs:range rdf:resource="#Collection"/>
    </owl:ObjectProperty>

</rdf:RDF>
