<rdf:RDF xmlns="http://clerezza.org/2009/09/hierarchy#"
	xml:base="http://clerezza.org/2009/09/hierarchy"
	xmlns:hierarchy="http://clerezza.org/2009/09/hierarchy#"
	xmlns:xsd="http://www.w3.org/2001/XMLSchema#"
	xmlns:rdfs="http://www.w3.org/2000/01/rdf-schema#"
	xmlns:rdf="http://www.w3.org/1999/02/22-rdf-syntax-ns#"
	xmlns:owl="http://www.w3.org/2002/07/owl#"
	xmlns:dc="http://purl.org/dc/elements/1.1/"
	xmlns:dbt="http://discobits.org/ontology#">

	<owl:Ontology rdf:about="http://clerezza.org/2009/09/hierarchy#">
		<dc:title>Clerezza Ontology for Hierarchical Structure</dc:title>
	</owl:Ontology>

    <!-- Classes -->

	<owl:Class rdf:about="#Collection">
		<rdfs:comment>An ordered  collection of members. The URI of a Collection
			must end with a slash ('/').</rdfs:comment>
	</owl:Class>

	<owl:Class rdf:about="#Page">
		<rdfs:comment>A titled content that is typically displayed in a web browser
			without being a part of a containing entity.</rdfs:comment>
		<rdfs:subClassOf rdf:resource="dbt:TitledContent" />
	</owl:Class>

	<owl:ObjectProperty rdf:about="#members">
        <rdfs:comment>Points to a list of Resources.</rdfs:comment>
        <rdfs:domain rdf:resource="#Collection"/>
        <rdfs:range rdf:resource="rdf:List"/>
    </owl:ObjectProperty>

	<owl:ObjectProperty rdf:about="#membersNumber">
        <rdfs:comment>Points from a collection to an integer that states the
			number of members in the collection.</rdfs:comment>
        <rdfs:domain rdf:resource="#Collection"/>
        <rdfs:range rdf:resource="xsd:int"/>
    </owl:ObjectProperty>

	<owl:ObjectProperty rdf:about="#parent">
        <rdfs:comment>Points from a resource to its parent collection.</rdfs:comment>
        <rdfs:range rdf:resource="#Collection"/>
    </owl:ObjectProperty>

</rdf:RDF>